draft: save progress

CoqOfRust/plonky3/blake3_air/links/columns.v
@@ -1,10 +1,13 @@
 Require Import CoqOfRust.CoqOfRust.
 Require Import CoqOfRust.links.M.
+Require Import core.links.array.
+Require Import plonky3.blake3_air.links.constants.
 Require Import plonky3.blake3_air.columns.
+
+Definition U32_LIMBS := links.constants.U32_LIMBS.
 
 (* TODO: 
 - check where is U32_LIMBS 
-- change `to_value` into concrete definition(?)
 *)
 
 (* 
@@ -29,8 +32,22 @@ pub(crate) struct QuarterRound<'a, T, U> {
     pub d_output: &'a [T; 32],
 }
 *)
+Module test.
+  Record t {T U : Set} `{Link T} `{Link U} : Set := {
+    a : Ref.t Pointer.Kind.Ref (array.t T U32_LIMBS); 
+  }.
+
+  Lemma of_value_with {T U : Set} `{Link T} `{Link U}
+    a a' :
+    a' = φ a -> Value.StructRecord "p3_blake3_air::columns::QuarterRound" [] [] [
+    ("a", a')
+    ] = φ (Build_t a).
+  Admitted.
+End test.
 Module QuarterRound.
-  Record t (T U : Set) : Set := {
+  (* NOTE: here we provide link instance for T and U or otherwise Coq cannot recognize
+  instances for arrays of them *)
+  Record t {T U : Set} `{Link T} `{Link U} : Set := {
     a : Ref.t Pointer.Kind.Ref (array.t T U32_LIMBS); 
     b : Ref.t Pointer.Kind.Ref (array.t T {| Integer.value := 32 |});
     c : Ref.t Pointer.Kind.Ref (array.t T U32_LIMBS); 
@@ -48,20 +65,153 @@ Module QuarterRound.
   }.
   Arguments t : clear implicits.
 
-  Parameter to_value : forall {T U : Set}, t T U -> Value.t.
-
-  Global Instance IsLink (T U : Set) `{Link T} `{Link U} : Link (t T U) := {
+  (* NOTE: the result from definition above is that it needs two extra Link instance for T and U here(???) *)
+  Global Instance IsLink (T U : Set) `{Link T} `{Link U} : Link (t T U _ _)
+  := {
     Φ := Ty.apply (Ty.path "p3_blake3_air::columns::QuarterRound") [] [ Φ T; Φ U ];
-    φ := to_value;
+    φ x :=
+      Value.StructRecord "p3_blake3_air::columns::QuarterRound" [] [] [
+        ("a", φ x.(a));
+        ("b", φ x.(b));
+        ("c", φ x.(c));
+        ("d", φ x.(d));
+        ("m_two_i", φ x.(m_two_i));
+        ("a_prime", φ x.(a_prime));
+        ("b_prime", φ x.(b_prime));
+        ("c_prime", φ x.(c_prime));
+        ("d_prime", φ x.(d_prime));
+        ("m_two_i_plus_one", φ x.(m_two_i_plus_one));
+        ("a_output", φ x.(a_output));
+        ("b_output", φ x.(b_output));
+        ("c_output", φ x.(c_output));
+        ("d_output", φ x.(d_output))
+      ];
   }.
 
   Definition of_ty (T_ty U_ty : Ty.t) :
     OfTy.t T_ty -> OfTy.t U_ty ->
     OfTy.t (Ty.apply (Ty.path "p3_blake3_air::columns::QuarterRound") [] [ T_ty ; U_ty ]).
-  Proof. intros [T] [U]. eapply OfTy.Make with (A := t T U). now subst. Defined.
+  Proof. intros [T] [U]. eapply OfTy.Make with (A := t T U _ _). now subst. Defined.
   Smpl Add eapply of_ty : of_ty.
-End QuarterRound.
 
+  (* 
+    Lemma of_value_with limit limit' remaining remaining' refunded refunded' memory memory' :
+    limit' = φ limit ->
+    remaining' = φ remaining ->
+    refunded' = φ refunded ->
+    memory' = φ memory ->
+    Value.StructRecord "revm_interpreter::gas::Gas" [] [] [
+      ("limit", limit');
+      ("remaining", remaining');
+      ("refunded", refunded');
+      ("memory", memory')
+    ] = φ (Build_t limit remaining refunded memory).
+  Proof. now intros; subst. Qed.
+  Smpl Add apply of_value_with : of_value.
+  *)
+
+  Lemma of_value_with {T U : Set} `{Link T} `{Link U}
+    a a'
+    b b'
+    c c'
+    d d'
+    m_two_i m_two_i'
+    a_prime a_prime'
+    b_prime b_prime'
+    c_prime c_prime'
+    d_prime d_prime'
+    m_two_i_plus_one m_two_i_plus_one'
+    a_output a_output'
+    b_output b_output'
+    c_output c_output'
+    d_output d_output' :
+      a' = φ a ->
+      b' = φ b ->
+      c' = φ c ->
+      d' = φ d ->
+      m_two_i' = φ m_two_i ->
+      a_prime' = φ a_prime ->
+      b_prime' = φ b_prime ->
+      c_prime' = φ c_prime ->
+      d_prime' = φ d_prime ->
+      m_two_i_plus_one' = φ m_two_i_plus_one ->
+      a_output' = φ a_output ->
+      b_output' = φ b_output ->
+      c_output' = φ c_output ->
+      d_output' = φ d_output ->
+    Value.StructRecord "p3_blake3_air::columns::QuarterRound" [] [] [
+      ("a", a');
+      ("b", b');
+      ("c", c');
+      ("d", d');
+      ("m_two_i", m_two_i');
+      ("a_prime", a_prime');
+      ("b_prime", b_prime');
+      ("c_prime", c_prime');
+      ("d_prime", d_prime');
+      ("m_two_i_plus_one", m_two_i_plus_one');
+      ("a_output", a_output');
+      ("b_output", b_output');
+      ("c_output", c_output');
+      ("d_output", d_output');
+    ] = φ (Build_t a b c d m_two_i a_prime b_prime c_prime d_prime 
+      m_two_i_plus_one a_output b_output c_output d_output).
+  Proof. now intros; subst. Qed.
+  Smpl Add apply of_value_with : of_value.
+
+  (* NOTE: for future reference, deleting link instances will report errors about undefined evars *)
+  Definition of_value {T U : Set} `{Link T} `{Link U}
+    (a : Ref.t Pointer.Kind.Ref (array.t T U32_LIMBS)) (a' : Value.t)
+    (b : Ref.t Pointer.Kind.Ref (array.t T {| Integer.value := 32|}))  (b' : Value.t)
+    (c : Ref.t Pointer.Kind.Ref (array.t T U32_LIMBS))  (c' : Value.t)
+    (d : Ref.t Pointer.Kind.Ref (array.t T {| Integer.value := 32|}))  (d' : Value.t)
+    (m_two_i : Ref.t Pointer.Kind.Ref (array.t U {| Integer.value := 32 |})) (m_two_i' : Value.t)
+    (a_prime : Ref.t Pointer.Kind.Ref (array.t T U32_LIMBS)) (a_prime' : Value.t)
+    (b_prime : Ref.t Pointer.Kind.Ref (array.t T {| Integer.value := 32 |})) (b_prime' : Value.t)
+    (c_prime : Ref.t Pointer.Kind.Ref (array.t T U32_LIMBS)) (c_prime' : Value.t)
+    (d_prime : Ref.t Pointer.Kind.Ref (array.t T {| Integer.value := 32 |})) (d_prime' : Value.t)
+    (m_two_i_plus_one : Ref.t Pointer.Kind.Ref (array.t U {| Integer.value := 32 |})) (m_two_i_plus_one' : Value.t)
+    (a_output : Ref.t Pointer.Kind.Ref (array.t T U32_LIMBS)) (a_output' : Value.t)
+    (b_output : Ref.t Pointer.Kind.Ref (array.t T {| Integer.value := 32 |})) (b_output' : Value.t)
+    (c_output : Ref.t Pointer.Kind.Ref (array.t T U32_LIMBS)) (c_output' : Value.t)
+    (d_output : Ref.t Pointer.Kind.Ref (array.t T {| Integer.value := 32 |})) (d_output' : Value.t)
+    :
+      a' = φ a ->
+      b' = φ b ->
+      c' = φ c ->
+      d' = φ d ->
+      m_two_i' = φ m_two_i ->
+      a_prime' = φ a_prime ->
+      b_prime' = φ b_prime ->
+      c_prime' = φ c_prime ->
+      d_prime' = φ d_prime ->
+      m_two_i_plus_one' = φ m_two_i_plus_one ->
+      a_output' = φ a_output ->
+      b_output' = φ b_output ->
+      c_output' = φ c_output ->
+      d_output' = φ d_output ->
+    OfValue.t (
+      Value.StructRecord "p3_blake3_air::columns::QuarterRound" [] [] [
+        ("a", a');
+        ("b", b');
+        ("c", c');
+        ("d", d');
+        ("m_two_i", m_two_i');
+        ("a_prime", a_prime');
+        ("b_prime", b_prime');
+        ("c_prime", c_prime');
+        ("d_prime", d_prime');
+        ("m_two_i_plus_one", m_two_i_plus_one');
+        ("a_output", a_output');
+        ("b_output", b_output');
+        ("c_output", c_output');
+        ("d_output", d_output')
+      ]
+    ).
+  Proof. econstructor; apply of_value_with; eassumption. Defined.
+  Smpl Add apply of_value : of_value.
+End QuarterRound.
+ 
 (* 
 pub struct Blake3State<T> {
     pub row0: [[T; U32_LIMBS]; 4],
@@ -79,11 +229,15 @@ Module Blake3State.
   }.
   Arguments t : clear implicits.
 
-  Parameter to_value : forall {T : Set}, t T -> Value.t.
-
-  Global Instance IsLink (T : Set) `{Link T} : Link (t T) := {
+  Global Instance IsLink (T U : Set) `{Link T} : Link (t T) := {
     Φ := Ty.apply (Ty.path "p3_blake3_air::columns::Blake3State") [] [ Φ T ];
-    φ := to_value;
+    φ x :=
+      Value.StructRecord "p3_blake3_air::columns::Blake3State" [] [] [
+        ("row0", φ x.(row0));
+        ("row1", φ x.(row1));
+        ("row2", φ x.(row2));
+        ("row3", φ x.(row3));
+      ];
   }.
 
   Definition of_ty (T_ty : Ty.t) :
@@ -91,6 +245,27 @@ Module Blake3State.
     OfTy.t (Ty.apply (Ty.path "p3_blake3_air::columns::Blake3State") [] [ T_ty ]).
   Proof. intros [T]. eapply OfTy.Make with (A := t T). now subst. Defined.
   Smpl Add eapply of_ty : of_ty.
+
+  Definition of_value {T : Set}
+    (row0 : array.t (array.t T U32_LIMBS) {| Integer.value := 4 |}) row0'
+    (row1 : array.t (array.t T {| Integer.value := 32 |}) {| Integer.value := 4 |}) row1'
+    (row2 : array.t (array.t T U32_LIMBS) {| Integer.value := 4 |}) row2'
+    (row3 : array.t (array.t T {| Integer.value := 32 |}) {| Integer.value := 4 |}) row3'
+    :
+    row0' = φ row0 ->
+    row1' = φ row1 ->
+    row2' = φ row2 ->
+    row3' = φ row3 ->
+    OfValue.t (
+      Value.StructRecord "p3_blake3_air::columns::Blake3State" [] [] [
+        ("row0", row0');
+        ("row1", row1');
+        ("row2", row2');
+        ("row3", row3');
+      ]
+    ).
+  Proof. econstructor; apply of_value_with; eassumption. Defined.
+  Smpl Add apply of_value : of_value.
 End Blake3State.
 
 (* 
@@ -110,11 +285,15 @@ Module FullRound.
   }.
   Arguments t : clear implicits.
 
-  Parameter to_value : forall {T : Set}, t T -> Value.t.
-
   Global Instance IsLink (T : Set) `{Link T} : Link (t T) := {
     Φ := Ty.apply (Ty.path "p3_blake3_air::columns::FullRound") [] [ Φ T ];
-    φ := to_value;
+    φ x :=
+      Value.StructRecord "p3_blake3_air::columns::FullRound" [] [] [
+        ("state_prime", φ x.(state_prime));
+        ("state_middle", φ x.(state_middle));
+        ("state_middle_prime", φ x.(state_middle_prime));
+        ("state_output", φ x.(state_output));
+      ];
   }.
 
   Definition of_ty (T_ty : Ty.t) :
@@ -122,4 +301,25 @@ Module FullRound.
     OfTy.t (Ty.apply (Ty.path "p3_blake3_air::columns::FullRound") [] [ T_ty ]).
   Proof. intros [T]. eapply OfTy.Make with (A := t T). now subst. Defined.
   Smpl Add eapply of_ty : of_ty.
+
+  Definition of_value {T : Set}
+    (state_prime : Blake3State.t T) state_prime'
+    (state_middle : Blake3State.t T) state_middle'
+    (state_middle_prime : Blake3State.t T) state_middle_prime'
+    (state_output : Blake3State.t T) state_output'
+  :
+    state_prime' = φ state_prime ->
+    state_middle' = φ state_middle ->
+    state_middle_prime' = φ state_middle_prime ->
+    state_output' = φ state_output ->
+    OfValue.t (
+      Value.StructRecord "p3_blake3_air::columns::FullRound"" [] [] [
+        ("state_prime", state_prime');
+        ("state_middle", state_middle');
+        ("state_middle_prime", state_middle_prime');
+        ("state_output", state_output');
+      ]
+    ).
+  Proof. econstructor; apply of_value_with; eassumption. Defined.
+  Smpl Add apply of_value : of_value.
 End FullRound.
